Update CFGProp.v

src/coq/CFGProp.v
@@ -1,8 +1,6 @@
-
 (* -------------------------------------------------------------------------- *
  *                     Vellvm - the Verified LLVM project                     *
  *                                                                            *
- *     Copyright (c) 2017 Dmitri Garbuzov <dgarbuzov@gmail.com>               *
  *     Copyright (c) 2017 Steve Zdancewic <stevez@cis.upenn.edu>              *
  *                                                                            *
  *   This file is distributed under the terms of the GNU General Public       *
@@ -10,364 +8,366 @@
  *   3 of the License, or (at your option) any later version.                 *
  ---------------------------------------------------------------------------- *)
 
-(** Reasoning about dominators in a graph. *)
-
-Require Import List Equalities Orders RelationClasses Omega.
-Require Import FSets FMaps.
+Require Import ZArith List String Omega.
+Require Import Vellvm.Ollvm_ast Vellvm.CFG Vellvm.Dom.
+Require Import Vellvm.Classes.
+Require Vellvm.AstLib.
 Import ListNotations.
-Require Import Vellvm.Util.
+Open Scope list_scope.
 
+(* invariants of the CFG machine -------------------------------------------- *)
 
-Module Type LATTICE.
-  Include EqLe'.
+Lemma incr_pc_in_block: forall CFG p1 p2, incr_pc CFG p1 = Some p2 -> (fn p1 = fn p2) /\ (bk p1 = bk p2).
+Proof.
+  intros CFG p1 p2 H.
+  unfold incr_pc in H.
+  destruct p1.
+  destruct (find_function CFG fn); simpl in H; try solve [inversion H].
+  destruct (find_block (blks (df_instrs d)) bk); simpl in H; try solve [inversion H].
+  destruct (block_to_cmd b pt); simpl in H; try solve [inversion H].
+  destruct p. destruct o; try inversion H.
+  simpl. split; reflexivity.
+Qed.  
 
-  Declare Instance eq_equiv : Equivalence eq.
-  Declare Instance le_preorder : PreOrder le.
-  Declare Instance le_poset : PartialOrder eq le.
+Lemma find_block_same_fid : forall CFG fid br phis p,
+    find_block_entry CFG fid br = Some (BlockEntry phis p) -> (fn p) = fid.
+Proof.
+  intros CFG fid br phis p H.
+  unfold find_block_entry in H.
+  destruct (find_function CFG fid); simpl in H; try solve [inversion H].
+  destruct (find_block (blks (df_instrs d)) br); simpl in H; try solve [inversion H].
+  destruct b. unfold block_to_entry in H. simpl in H. inversion H.
+  simpl. reflexivity.
+Qed.  
   
-  Parameter eq_dec : forall x y, {x == y} + {x ~= y}.
-
-  Parameter bot : t.
-  Axiom le_bot : forall x, bot <= x.
-
-  Parameter top : t.
-  Axiom le_top : forall x, x <= top.
-
-  Parameter join : t -> t -> t.
-  Axiom le_join_l : forall x y, x <= join x y.
-  Axiom le_join_r : forall x y, y <= join x y.
-End LATTICE.
-
-Module BoundedSet(Import S:FSetInterface.WS) <: LATTICE.
-
-  Module Import SFacts := FSetFacts.WFacts S.
-
-  Definition t : Type := option S.t.
-
-  Definition eq (t1 t2: t) : Prop :=
-    match t1, t2 with
-      | Some s1, Some s2 => s1 [=] s2
-      | None, None => True
-      | _, _ => False
-    end.
-
-  Definition le (t1 t2: t) : Prop :=
-    match t1, t2 with
-      | Some s1, Some s2 => s2 [<=] s1
-      | None, Some _ | None, None => True
-      | Some _, None => False
-    end.
-
-  Include EqLeNotation.
-
-  Instance eq_equiv : Equivalence eq.
-  Proof.
-    constructor.
-    red. destruct x; simpl; intuition.
-    red. destruct x, y; simpl; intros; intuition.
-    red. destruct x, y, z; simpl; intros; intuition.
-    transitivity t1; auto.
-  Qed.
-
-  Instance le_preorder : PreOrder le.
-  Proof.
-    constructor.
-    red. destruct x; simpl; intuition. 
-    red. destruct x, y, z; simpl; intros; intuition.
-    transitivity t1; auto.
-  Qed.
-
-  Instance le_poset : PartialOrder eq le.
-  Proof.
-    constructor.
-    intro. repeat red. split.
-    destruct x, x0; simpl in *; intuition. 
-    unfold Subset. intros. rewrite H; auto.
-    red. destruct x, x0; simpl in *; intuition.
-    unfold Subset. intros. rewrite <- H. auto.
-
-    destruct x, x0; simpl; 
-      intros H; repeat red in H; simpl in H; 
-      intuition.
-    repeat red in H1. repeat red in H0.
-    red; intuition.
-  Qed.
-
-  Definition eq_dec : forall x y, {x == y} + {x ~= y}.
-    refine (fun t1 t2 => match t1, t2 with
-                           | Some s1, Some s2 => _
-                           | None, None => left _
-                           | _, _ => right _
-                         end); auto using S.eq_dec.
-  Defined.
-
-  Definition bot : t := None.
-
-  Lemma le_bot : forall x, bot <= x.
-  Proof.
-    simpl; destruct x; trivial.
-  Qed.
-
-  Definition top : t := Some S.empty.
-  Lemma le_top : forall x, x <= top.
-  Proof. 
-    simpl. destruct x; trivial. red. intros.
-    exfalso. eapply empty_iff; eauto. 
-  Qed.
-
-  Definition join (t1 t2: t) : t :=
-    match t1, t2 with
-      | Some s1, Some s2 => Some (S.inter s1 s2) 
-      | None, Some s | Some s, None => Some s
-      | None, None => None
-    end.
-
-  Lemma le_join_l : forall x y, x <= join x y.
-  Proof.
-    intros. destruct x, y; repeat red; auto.
-    intros. eapply inter_1; eauto.
-  Qed.
-
-  Lemma le_join_r : forall x y, y <= join x y.
-  Proof.
-    intros. destruct x, y; repeat red; auto.
-    intros. eapply inter_2; eauto.
-  Qed.
-
-  Definition union (t1 t2: t) : t :=
-    match t1, t2 with
-      | Some s1, Some s2 => Some (S.union s1 s2) 
-      | None, Some s | Some s, None => None
-      | None, None => None
-    end.
     
-  Definition singleton (e:S.elt) : t := Some (S.singleton e).
 
-  Definition In (e:S.elt) (t:t) : Prop :=
-    match t with
-      | Some s => S.In e s
-      | None => True
-    end.
+(* syntactic structure ------------------------------------------------------ *)
 
-End BoundedSet.
+Inductive CFG_has_code_at (CFG:mcfg) (P:pc -> Prop) : pc -> code -> Prop :=
+| has_code_nil :
+    forall p, P p -> CFG_has_code_at CFG P p []
+| has_code_cons :
+    forall p iid instr pc_next cd
+      (HF: fetch CFG p = Some (Step instr))
+      (Hiid: (pt p) = iid)
+      (Hincr: incr_pc CFG p = Some pc_next)
+      (Hcd: CFG_has_code_at CFG P pc_next cd),
+      CFG_has_code_at CFG P p ((iid,instr)::cd).
+Hint Constructors CFG_has_code_at.
+
+Lemma CFG_has_code_app :
+  forall CFG P (cd1 cd2:code) (pc1 pc2:pc)
+    (H1: CFG_has_code_at CFG (fun p => p = pc2) pc1 cd1)
+    (H2: CFG_has_code_at CFG P pc2 cd2),
+    CFG_has_code_at CFG P pc1 (cd1 ++ cd2).
+Proof.
+  intros CFG P cd1 cd2 pc1 pc2 H1.
+  remember (fun p => p = pc2) as Q.
+  revert cd2.
+  induction H1; intros cd2 H2; simpl in *; auto.
+  - subst. subst. auto.
+  - eapply has_code_cons; eauto.
+Qed.    
+
+Lemma CFG_has_code_app_inv :
+  forall CFG P pc1 (cd1 cd2:code)
+    (H:CFG_has_code_at CFG P pc1 (cd1 ++ cd2)),
+  exists pc2,
+    CFG_has_code_at CFG (fun p => p = pc2) pc1 cd1 /\
+    CFG_has_code_at CFG P pc2 cd2.
+Proof.
+  intros CFG P pc1 cd1.
+  revert pc1.
+  induction cd1; intros pc1 cd2 H; inversion H; subst; simpl in *; auto.
+  - exists pc1. split; eauto.
+  - exists pc1. subst. split; eauto.
+  - apply IHcd1 in Hcd.
+    destruct Hcd as [pc2 [HA HB]].
+    exists pc2. split; eauto.
+Qed.
 
 
+Definition CFG_has_pc (CFG:mcfg) (p:pc) : Prop :=
+  exists cmd, fetch CFG p = Some cmd.
 
-(** ** GRAPH *)
-(** Interface for a nonempty graph [t] with: 
-     - a set of _vertices_ of type [V]
-     - a distinguished _entry vertex_
-     - an _edge relation_ [edge]
+Definition CFG_fun_has_block_id (CFG:mcfg) (fid:function_id) (bid:block_id) phis (p:pc) : Prop :=
+  find_block_entry CFG fid bid = Some (BlockEntry phis p) /\ CFG_has_pc CFG p. 
+
+
+Inductive CFG_fun_has_terminator_lbls (CFG:mcfg) (fid:function_id) : terminator -> Prop :=
+| lbls_Ret : forall v, CFG_fun_has_terminator_lbls CFG fid (TERM_Ret v)
+| lbls_Ret_void : CFG_fun_has_terminator_lbls CFG fid TERM_Ret_void
+| lbls_TERM_Br :
+    forall v br1 phis1 p1 br2 phis2 p2
+      (Hbr1 : CFG_fun_has_block_id CFG fid br1 phis1 p1)
+      (Hbr2 : CFG_fun_has_block_id CFG fid br2 phis2 p2),
+      CFG_fun_has_terminator_lbls CFG fid (TERM_Br v br1 br2)
+| lbls_TERM_Br_1 :
+    forall br phis p
+      (Hbr : CFG_fun_has_block_id CFG fid br phis p),
+      CFG_fun_has_terminator_lbls CFG fid (TERM_Br_1 br)
+| lbls_Resume : forall v, CFG_fun_has_terminator_lbls CFG fid (TERM_Resume v)
+.
+(* TODO:  Add these cases:
+  | TERM_Switch     (v:tvalue) (default_dest:block_id) (brs: list (tvalue * block_id))
+  | TERM_IndirectBr 
+  | TERM_Invoke     (fnptrval:tident) (args:list tvalue) (to_label:block_id) (unwind_label:block_id)
+  .
 *)
 
-Module Type GRAPH.
-  Parameter Inline t V : Type.
-  Parameter Inline eq_dec_V : forall (v1 v2:V), {v1 = v2} + {v1 <> v2}.  
-  Parameter Inline entry : t -> V.
-  Parameter Inline edge : t -> V -> V -> Prop.
-  Parameter Inline mem : t -> V -> Prop.
-End GRAPH.
 
-(** ** Specification of Dominators *)
+Inductive CFG_has_terminator_at (CFG:mcfg) : pc -> instr_id -> terminator -> Prop :=
+| CFG_has_termintator_intro :
+    forall p iid t
+      (HF: fetch CFG p = Some (Term t))
+      (Hiid: (pt p) = iid)
+      (Hbrs: CFG_fun_has_terminator_lbls CFG (fn p) t),
+      CFG_has_terminator_at CFG p iid t.
 
-Module Spec (Import G:GRAPH).
 
-(** Defines a path in the graph. *)
+Inductive CFG_fun_has_block (CFG:mcfg) (fid:function_id) (b:block) phis : Prop :=
+| CFG_fun_has_block_intro:
+    forall
+      (HFind: find_block_entry CFG fid (blk_id b) = Some (BlockEntry phis (blk_entry_pc fid b)))      
+      (Hcode: CFG_has_code_at CFG (fun q => q = blk_term_pc fid b) (blk_entry_pc fid b) (blk_code b))
+      (Hterm: CFG_has_terminator_at CFG (blk_term_pc fid b) (blk_term_id b) (blk_terminator b))
+    ,
+      CFG_fun_has_block CFG fid b phis.
 
-  Inductive Path (g:G.t) : V -> V -> list V -> Prop :=
-  | path_nil : forall v, 
-      mem g v -> Path g v v [v]
-  | path_cons : forall v1 v2 v3 vs,
-      Path g v1 v2 vs -> mem g v3 -> edge g v2 v3 
-      -> Path g v1 v3 (v3::vs).
 
-Hint Constructors Path.
+Definition CFG_fun_has_blocks (CFG:mcfg) (fid:function_id) (bs:list block) : Prop :=
+  Forall (fun b => exists phis, CFG_fun_has_block CFG fid b phis /\ CFG_fun_has_terminator_lbls CFG fid (snd (blk_term b))) bs.
+
+
+(* well formedness ---------------------------------------------------------- *)
+(*
+(* When does a cfg program point define a given local_id. *)
+Definition pt_defines (p:pt) (lid:local_id) :=
+  match p with
+  | IId id => if id == lid then True else False
+  | IVoid _ => False
+  end.
+*)
+
+(* Which identifiers does an instruction use? *)
+Fixpoint value_uses (v:value) : list ident :=
+  match v with
+  | SV (VALUE_Ident id) => [id]
+  | SV (VALUE_Integer _)
+  | SV (VALUE_Float _ )
+  | SV (VALUE_Bool _)
+  | SV (VALUE_Null)
+  | SV (VALUE_Zero_initializer)
+  | SV (VALUE_Cstring _)
+  | SV (VALUE_None)
+  | SV (VALUE_Undef) => []
+
+  | SV (VALUE_Struct l)
+  | SV (VALUE_Packed_struct l)
+  | SV (VALUE_Array l)
+  | SV (VALUE_Vector l) => List.flat_map (fun x => value_uses (snd x)) l
+  | SV (OP_IBinop _ _ v1 v2) 
+  | SV (OP_ICmp _ _ v1 v2)
+  | SV (OP_FBinop _ _ _ v1 v2) 
+  | SV (OP_FCmp _ _ v1 v2) => (value_uses v1) ++ (value_uses v2)
+  | SV (OP_Conversion _ _ v _) => value_uses v
+  | SV (OP_GetElementPtr _ (_,ptr) idxs) => (value_uses ptr) ++ (List.flat_map (fun x => value_uses (snd x)) idxs)
+  | SV (OP_ExtractElement  (_,vec) (_,idx)) => (value_uses vec) ++ (value_uses idx)
+  | SV (OP_InsertElement (_,vec) (_,elt) (_,idx)) => (value_uses vec) ++ (value_uses elt) ++ (value_uses idx)
+  | SV (OP_ShuffleVector (_, vec1) (_,vec2) (_,idxmask)) => (value_uses vec1) ++ (value_uses vec2) ++ (value_uses idxmask)
+  | SV (OP_ExtractValue (_,vec) _) => value_uses vec
+  | SV (OP_InsertValue (_,vec) (_,elt) _) => (value_uses vec) ++ (value_uses elt)
+  | SV (OP_Select (_,cnd) (_,v1) (_,v2)) => (value_uses cnd) ++ (value_uses v1) ++ (value_uses v2)
+  end.
+
+Definition tvalue_uses (tv:tvalue) : list ident := value_uses (snd tv).
+
+Definition phi_uses (i:phi) : (list ident) :=
+  match i with
+  | Phi  t args => List.flat_map (fun x => value_uses (snd x)) args
+  end.
+
+(* over-approximation: may include the same identifier more than once *)
+Definition instr_uses (i:instr) : (list ident) :=
+  match i with
+  | INSTR_Op op => value_uses op                         
+  | INSTR_Call (_, fid) args => [fid] ++ (List.flat_map tvalue_uses args)
+  | INSTR_Alloca t None align => []
+  | INSTR_Alloca t (Some tv) align => tvalue_uses tv
+  | INSTR_Load  volatile t ptr align => tvalue_uses ptr
+  | INSTR_Store volatile val ptr align => (tvalue_uses val) ++ (tvalue_uses ptr)
+  | INSTR_Fence 
+  | INSTR_AtomicCmpXchg
+  | INSTR_AtomicRMW
+  | INSTR_Unreachable
+  | INSTR_VAArg
+  | INSTR_LandingPad => []
+  end.
+
+Definition terminator_uses (t:terminator) : list ident :=
+  match t with
+  | TERM_Ret tv => tvalue_uses tv
+  | TERM_Ret_void => []
+  | TERM_Br tv _ _ => tvalue_uses tv
+  | TERM_Br_1  _ => []
+  | TERM_Switch  tv _ brs => (tvalue_uses tv) ++ (List.flat_map (fun x => tvalue_uses (fst x)) brs)
+  | TERM_IndirectBr tv _ => tvalue_uses tv
+  | TERM_Resume tv => tvalue_uses tv
+  | TERM_Invoke (_,fid) args _ _ => [fid] ++ (List.flat_map tvalue_uses args)
+  end.
+
+(*
+Definition cmd_uses_local (g:cfg) (p:pt) (id:local_id) : Prop :=
+  match (code g) p with
+  | Some (Step ins _) => In (ID_Local id) (instr_uses ins)
+  | Some (Jump _ t) => In (ID_Local id) (terminator_uses t)
+  | None => False
+  end.
+*)             
+
+(* Which labels does a terminator mention *)
+Definition lbls (t:terminator) : list block_id :=
+  match t with
+  | TERM_Ret _        
+  | TERM_Ret_void   => []
+  | TERM_Br _ l1 l2 => [l1; l2] 
+  | TERM_Br_1 l => [l] 
+  | TERM_Switch _ l brs => l::(List.map (fun x => snd x) brs)
+  | TERM_IndirectBr _ brs => brs
+  | TERM_Resume _    => []
+  | TERM_Invoke  _ _ l1 l2 => [l1; l2] 
+  end.
+
+(*
+(* Well-formed SSA-form CFGs 
+   - the initial pt denotes a command  
+   - fallthrough closure: each fallthrough pt maps to a command 
+   - jump closure: each label used in a terminator leads to a
+     block within the same function body.
+   - every use of an identifier is dominated by the id's definition
+   - no identifier is defined multiple times
+*)
+Definition pt_exists (CFG : cfg) (p:pt) : Prop :=
+  exists cmd, (code CFG p) = Some cmd.
+(** Edge relation *)
+Inductive edge_pt (g:cfg) : pt -> pt -> Prop :=
+| edge_pt_S : forall p i q,
+    (code g) p = Some (Step i q) ->
+    edge_pt g p q
+| edge_pt_J : forall p b t l q xs r,
+    (code g) p = Some (Jump b t) ->
+    In l (lbls t) ->
+    (phis g) l = Some (Phis q xs r) ->
+    edge_pt g p q.
+(** *** GRAPH instance for dominance calculation *)
+(** Graph of program points *)
+Module PtGraph <: GRAPH.
+  Definition t := cfg.
+  Definition V := pt.
+  Definition entry g := init g.
+  Definition edge := edge_pt.
+  Definition mem := pt_exists.
+  Definition eq_dec_V := AstLib.eq_dec_instr_id.
+End PtGraph.
+Module Export Dom := Dom.Spec PtGraph.
+(** *** Definitions for Well-formed SSA programs. *)
+(** Most of the LLVM instructions define the uid associated
+  with their program point.  Some (like [store], [void] calls, and the [terminator]s)
+  do not. *)
+Definition def_at_pt (g:cfg) (p:pt) (lid:local_id) : Prop :=
+  pt_exists g p /\ pt_defines p lid.
+(** The definition of id dominates its use at point pt *)
+Inductive well_scoped_use_at_pt (g:cfg) (p:pt) : ident -> Prop :=
+| ws_global : forall id, In id (glbl g) -> pt_exists g p -> well_scoped_use_at_pt g p id
+| ws_local : forall lid p', def_at_pt g p' lid -> SDom g p' p -> well_scoped_use_at_pt g p (ID_Local lid).
+(** All uses of a [uid] must be strictly dominated by their definitions. *)
+Definition wf_use (g:cfg) (ids:list ident) (p:pt) : Prop :=
+  forall id, In id ids -> well_scoped_use_at_pt g p id.
+(** *** Well-formed phi nodes *)
+(**  Consider [ %x = phi [lbl1:v1, ...,lbln:vn] ].  This is well formed
+     when every predecessor block with terminator program point p' 
+     has a label associated with value v.  Moreover, if v uses an id then
+     the definition of the uid strictly dominates p'.
+*)
+Definition wf_phi_args (g:cfg) (entry:pt) (args:list (block_id * value)) :=
+  forall pred, edge_pt g pred entry ->
+          exists b t, (code g) pred = Some (Jump b t) /\
+                 exists v, In (b,v) args /\ wf_use g (value_uses v) pred.
+Inductive wf_phis (CFG : cfg) (entry:pt) (q : pt) : pt -> list (local_id * instr) -> Prop :=
+| wf_phis_nil : pt_exists CFG q ->
+                wf_phis CFG entry q q []
+| wf_phis_cons :
+    forall p p' x t args rest,
+    (code CFG p) = Some (Step (INSTR_Phi t args) p') ->
+    wf_phi_args CFG entry args ->
+    wf_phis CFG entry q p' rest ->
+    wf_phis CFG entry q p ((x, INSTR_Phi t args) :: rest) .
+Inductive wf_cmd (g:cfg) (p:pt) : cmd -> Prop :=
+| wf_step : forall (i:instr) (q:pt)
+              (Hq : pt_exists g q)
+              (Huse: wf_use g (instr_uses i) p),
+    wf_cmd g p (Step i q)
+| wf_jump : forall (bn:block_id) (t:terminator)
+              (Huse: wf_use g (terminator_uses t) p)
+              (Hlbls: Forall (fun tgt => exists p', exists xs, exists q,
+                             (phis g tgt) = Some (Phis p' xs q) 
+                             /\ wf_phis g p' q p' xs
+                      )
+                      (lbls t)),
+    wf_cmd g p (Jump bn t).
+(* TODO: do we have to worry about locals shadowing function parameters? 
+   Could add: forall lid, In (ID_Local lid) (glbl CFG) -> (code CFG) (IId lid) = None
+   - also, somewhere probably need that globals and function parameters are distinct
+ *)
+Definition wf_cfg (CFG : cfg) : Prop :=
+  pt_exists CFG (init CFG)
+  /\ forall p, ~ edge_pt CFG p (init CFG)            
+  /\ (forall p cmd, (code CFG p) = Some cmd -> wf_cmd CFG p cmd)
+.
+            
+Lemma wf_cfg_edge_pt : forall g p1 p2,
+    wf_cfg g -> pt_exists g p1 -> edge_pt g p1 p2 -> pt_exists g p2.
+Proof.
+  intros g p1 p2 H H0 H1.
+  destruct H as [Hinit [Hintro Hcmd]].
+  inversion H1; subst.
+  - apply Hcmd in H. inversion H. exact Hq.
+  - apply Hcmd in H.
+    inversion H. subst. 
+    eapply Forall_forall in Hlbls.
+    Focus 2. apply H2.
+    destruct Hlbls as [p' [xs' [q [Ha Hb]]]].
+    rewrite H3 in Ha. inversion Ha. subst.
+    induction Hb.
+    * exact H4.
+    * exists (Step (INSTR_Phi t0 args) p'0).
+      exact H4.
+Unshelve. auto.
+Qed.      
+(* domination trees --------------------------------------------------------- *)
+  (* Quite hard to prove this:
+      - need to know that Dom can be definied equivalently by quantifying over 
+        all acyclic paths from entry
+      - need to know that there are a finite number of acyclic paths (and hence can
+        be enumerated)  DFS
+      - would work better with adjacency list representation of the graph
+  *)
+  Lemma dom_dec : forall (g:cfg) (v1 v2 : pt), {Dom g v1 v2} + {~Dom g v1 v2}.
+  Proof.
+    intros g v1 v2.
+  Admitted.
   
-(** *** Definition of domination *)
-
-  Definition Dom (g:G.t) (v1 v2: V) : Prop :=
-    forall vs, Path g (entry g) v2 vs -> In v1 vs.
-
-  Definition SDom (g:G.t) (v1 v2 : V) : Prop :=
-    v1 <> v2 /\ Dom g v1 v2.
-
-  Definition IDom (g:G.t) (v1 v2 : V) : Prop :=
-    SDom g v1 v2 /\ forall v3, SDom g v3 v2 -> Dom g v3 v1.
-
-  Definition reachable (g:G.t) (v : V) : Prop :=
-    exists p, Path g (entry g) v p.
-
-
-  Lemma start_in_path: forall (g:G.t) (v1 v2 : V) p,
-      Path g v1 v2 p -> In v1 p.
-  Proof.
-    intros g v1 v2 p H.
-    induction H.
-    - simpl. left. reflexivity.
-    - simpl. right. exact IHPath.
-  Qed.
-
+  Inductive vtree (A:Type) : Type :=
+  | vnode (v:A) (cs:list (vtree A)).
+  Arguments vnode {A} _ _.
   
-  Lemma end_in_path: forall (g:G.t) (v1 v2 : V) p,
-      Path g v1 v2 p -> In v2 p.
-  Proof.
-    intros g v1 v2 p H.
-    destruct H; left; reflexivity.
-  Qed.
-    
-  Lemma acyclic_path_exists: forall (g:G.t) (v1 v2 v3 : V) p,
-      Path g v1 v2 p -> In v3 p -> exists q, Path g v1 v3 (v3::q) /\ ~ In v3 q.
-  Proof.
-    intros g v1 v2 v3 p Hp Hin.
-    generalize dependent v3.
-    induction Hp; simpl; intros u Hin.
-    - destruct Hin. subst. exists []. split.
-      * apply path_nil. exact H.
-      * simpl. auto.
-      * inversion H0.
-    - destruct Hin. subst.
-      * destruct (in_dec eq_dec_V u vs).
-      + apply IHHp in i. exact i.
-      + exists vs. split. eapply path_cons; eauto. auto.
-      * apply IHHp in H1. exact H1.
-  Qed.            
-
-  Lemma path_splits: forall (g:G.t) (v1 v2 v3 : V) p,
-      Path g v1 v2 p -> In v3 p ->
-      exists p1, exists p2, Path g v1 v3 (v3::p1)
-                  /\ Path g v3 v2 (v2::p2)
-                  /\ p = (v2::p2 ++ p1).
-  Proof.
-    intros g v1 v2 v3 p Hp Hin.
-    generalize dependent v3.
-    induction Hp; simpl; intros u Hin.
-    - destruct Hin. subst.
-      * exists []. exists []. repeat split;auto.
-      * destruct H0.
-    - destruct Hin. subst.
-      * exists vs. exists []. split.
-        eapply path_cons; eauto.
-        split. apply path_nil; eauto. simpl. reflexivity.
-      * eapply IHHp in H1.
-        destruct H1 as [p1 [p2 [Hp1 [Hp2 Heq]]]].
-        exists p1. exists (v2::p2). split; auto. split.
-        eapply path_cons; eauto. subst. reflexivity.
-  Qed.        
-
-  Lemma Dom_reflexive : forall (g:G.t) (v : V),
-      Dom g v v.
-  Proof.
-    intros g v.
-    unfold Dom.
-    intros vs Hp.
-    eapply end_in_path. apply Hp.
-  Qed.
-  
-  Lemma Dom_antisymmetric : forall (g:G.t) (v1 v2 : V),
-      reachable g v1 -> 
-      Dom g v1 v2 -> Dom g v2 v1 -> v1 = v2.
-  Proof.
-    intros g v1 v2 H1 D1 D2.
-    unfold Dom in *.
-    destruct H1 as [p Hp].
-    assert (In v1 p). eapply end_in_path. apply Hp.
-    destruct (acyclic_path_exists g (entry g) v1 v1 p Hp H) as [p' [Hp' Hin]].
-    assert (In v2 (v1 :: p')) as Hin'. eapply D2. apply Hp'.
-    destruct (path_splits g (entry g) v1 v2 (v1::p') Hp' Hin') as [q1 [q2 [HQ1 [HQ2 Heq]]]].
-    inversion Heq. subst. clear Heq.
-    eapply D1 in HQ1.
-    destruct (in_inv HQ1). auto.
-    contradiction Hin. eapply in_or_app. right. apply H0.
-  Qed.
-
-  Lemma Dom_transitive : forall (g:G.t) (v1 v2 v3 : V),
-      Dom g v1 v2 -> Dom g v2 v3 -> Dom g v1 v3.
-  Proof.
-    intros g v1 v2 v3 D1 D2.
-    unfold Dom in *.
-    intros vs Hp.
-    destruct (path_splits g (entry g) v3 v2 vs) as [q1 [q2 [HQ1 [HQ2 Heq]]]]; auto. 
-    apply D1 in HQ1.
-    inversion HQ1.
-    - subst. rewrite app_comm_cons.
-      apply in_or_app. left. eapply start_in_path. apply HQ2.
-    - subst. simpl. right. apply in_or_app. right. exact H.
-  Qed.
-    
-  Lemma IDom_unique : forall (g:G.t) (v1 v2 v : V),
-      reachable g v1 ->
-      IDom g v1 v -> IDom g v2 v -> v1 = v2.
-  Proof.
-    intros g v1 v2 v H H1 H2.
-    destruct H1 as [S1 H1].
-    destruct H2 as [S2 H2].
-    apply H1 in S2.
-    apply H2 in S1.
-    eapply Dom_antisymmetric; eauto.
-  Qed.
-  
-    
-  Lemma dom_step : forall g v1 v2,
-    mem g v2 -> edge g v1 v2 -> forall v', SDom g v' v2 -> Dom g v' v1.
-  Proof.
-    unfold SDom, Dom. intros g v1 v2 Hmem Hsucc v' [Hneq Hdom] p Hp.
-    cut (In v' (v2::p)). inversion 1; subst; intuition. 
-    apply Hdom. eapply path_cons; eauto. 
-  Qed.
-
-End Spec.
-
-(** *** Relate an algorithm to the specification *)
-Module Type Algdom (Import G:GRAPH).
-  Module Import GS := Spec G.
-
-  Declare Module E : UsualDecidableType with Definition t := V.
-  Declare Module NS : FSetInterface.WS with Module E:=E.
-  Module L := BoundedSet NS.
-  Include EqLeNotation L.
-
-  Parameter calc_sdom : G.t -> option (V -> L.t).
-
-  Axiom entry_sound : forall g sdom,
-    calc_sdom g = Some sdom ->
-    sdom (entry g) == L.top.
-
-  Axiom successors_sound : forall g sdom n1 n2,
-    calc_sdom g = Some sdom ->
-    mem g n1 -> mem g n2 -> edge g n1 n2 -> 
-    L.union (L.singleton n1) (sdom n1) <= sdom n2.
-
-  Axiom complete : forall g sdom n1 n2,
-    calc_sdom g = Some sdom ->
-    SDom g n1 n2 -> L.In n1 (sdom n2).
-
-End Algdom.
-
-Module AlgdomProperties (Import G:GRAPH) (Import A : Algdom G).
-  Module Import GS := Spec G.
-
-  Lemma sound : forall g sdom n1 n2,
-    calc_sdom g = Some sdom ->              
-    L.In n1 (sdom n2) -> Dom g n1 n2.
-  Proof.
-    red; intros. remember (entry g). induction H1. subst.
-    pose proof entry_sound g sdom H. 
-
-    destruct (sdom (entry g)); try contradiction; simpl in *.
-      exfalso. rewrite H2 in H0. eapply L.SFacts.empty_iff. eauto.
-      
-    right. destruct (E.eq_dec v2 n1). subst. inversion H1; intuition.
-    apply IHPath; auto.
-
-    destruct (sdom v2) eqn:Heqv2; simpl in *; auto.
-    cut (NS.In n1 (NS.union (NS.singleton v2) t0)).
-    intro Hin. apply NS.union_1 in Hin as [Hin | Hin]; auto.
-    contradict n. apply NS.singleton_1. assumption.
-
-    pose proof successors_sound g sdom v2 v3 as Hss.
-    simpl in Hss. rewrite Heqv2 in Hss. simpl in Hss.
-    destruct (sdom v3). apply Hss; inversion H1; eauto.
-    exfalso. apply Hss; inversion H1; eauto.
-  Qed.
-
-End AlgdomProperties.
+  Inductive dom_tree (g:cfg) : instr_id -> (vtree instr_id) -> Prop :=
+  | dom_tree_intro:
+      forall (v:instr_id) (cs:list (vtree instr_id)), 
+        (forall u, IDom g v u -> exists (t:vtree instr_id), In t cs /\ dom_tree g u t) ->
+        (forall t, In t cs -> exists u, IDom g v u /\ dom_tree g u t) ->
+        dom_tree g v (vnode v cs). 
+  Lemma dom_tree_exists : forall (g:cfg), exists (t:vtree instr_id), dom_tree g (init g) t.
+  Admitted.
+*)
